Add anti renaming

theories/par.v
@@ -1,4 +1,4 @@
-Require Import Autosubst2.syntax unscoped core FunInd ssreflect.
+Require Import Autosubst2.syntax unscoped core FunInd ssreflect ssrbool.
 From Hammer Require Import Tactics.
 From stdpp Require Import relations (rtc(..)).
 
@@ -128,3 +128,111 @@ Qed.
 Lemma Par_subst a0 a1 (h : a0 ⇒ a1) σ :
   (subst_Tm σ a0 ⇒ subst_Tm σ a1).
 Proof. hauto l:on use:Par_refl, Par_morphing. Qed.
+
+
+(* Identifying neutral (ne) and normal (nf) terms *)
+Fixpoint ne (a : Tm) : bool :=
+  match a with
+  | VarTm _ => true
+  | App a b => ne a && nf b
+  | Abs _ => false
+  | Pi A B => false
+  | Univ _ => false
+  | Empty => false
+  | Squash _ => false
+  | Absurd a => nf a
+  | Box _ => false
+  | Let a b => ne a && nf b
+  end
+with nf (a : Tm) : bool :=
+  match a with
+  | VarTm _ => true
+  | App a b => ne a && nf b
+  | Abs _ => false
+  | Pi A B => nf A && nf B
+  | Univ _ => true
+  | Empty => true
+  | Squash A => nf A
+  | Absurd a => nf a
+  | Box a => nf a
+  | Let a b => ne a && nf b
+  end.
+
+Definition wn a := exists b, rtc Par a b /\ nf b.
+Definition wne a := exists b, rtc Par a b /\ ne b.
+
+Lemma ne_nf a : ne a -> nf a.
+Proof. elim : a =>//; hauto q:on unfold:nf inv:Par. Qed.
+
+Lemma wne_wn a : wne a -> wn a.
+Proof. sfirstorder use:ne_nf. Qed.
+
+Lemma nf_wn v : nf v -> wn v.
+Proof. sfirstorder ctrs:rtc. Qed.
+
+Lemma ne_nf_renaming a ξ :
+    (ne a <-> ne (ren_Tm ξ a)) /\ (nf a <-> nf (ren_Tm ξ a)).
+Proof.
+  elim : a ξ; solve [auto; hauto b:on].
+Qed.
+
+Lemma nf_refl a b (h: a ⇒ b) : (nf a -> b = a) /\ (ne a -> b = a).
+Proof.
+  elim : a b / h => // ; hauto b:on.
+Qed.
+
+Lemma nf_refl_star a b (h: rtc Par a b) : (nf a -> b = a) /\ (ne a -> b = a).
+Proof.
+  induction h; hauto lq:on rew:off inv:Tm ctrs:rtc use:nf_refl.
+Qed.
+
+Lemma nf_ne_preservation a b (h : a ⇒ b) : (nf a ==> nf b) /\ (ne a ==> ne b).
+Proof.
+  elim : a b / h => //; hauto lqb:on depth:2.
+Qed.
+
+Lemma nf_preservation : forall a b, (a ⇒ b) -> nf a -> nf b.
+Proof. sfirstorder use:nf_ne_preservation b:on. Qed.
+
+Lemma ne_preservation : forall a b, (a ⇒ b) -> ne a -> ne b.
+Proof. sfirstorder use:nf_ne_preservation b:on. Qed.
+
+Create HintDb nfne.
+#[export]Hint Resolve nf_wn ne_nf wne_wn ne_preservation nf_preservation : nfne.
+
+Lemma Par_antirenaming a b0 ξ
+  (h : ren_Tm ξ a ⇒ b0) : exists b, (a ⇒ b) /\ b0 = ren_Tm ξ b.
+Proof.
+  move E : (ren_Tm ξ a) h => a0 h.
+  move : a ξ E.
+  elim : a0 b0 /h.
+  - move => + []//=. hauto lq:on ctrs:Par.
+  - move => n []//=. hauto lq:on ctrs:Par.
+  - move => + + + + + + + + []//=. hauto lq:on ctrs:Par.
+  - move => + + + + []//=. hauto lq:on ctrs:Par.
+  - move => + + + + + + + + []//=. hauto lq:on ctrs:Par.
+  - move => a a0 b0 b1 ha iha hb ihb []//=.
+    move => []//= t t0 ξ [*]. subst.
+    specialize iha with (1 := eq_refl).
+    specialize ihb with (1 := eq_refl).
+    move : iha => [t'][? ?]. subst.
+    move : ihb => [t0'][? ?]. subst.
+    eexists. split.
+    by eauto using P_AppAbs.
+    by asimpl.
+  - hauto q:on ctrs:Par inv:Tm.
+  - hauto q:on ctrs:Par inv:Tm.
+  - move => + + + + + + + + []//=.
+    hauto lq:on ctrs:Par.
+  - move => a0 a1 b0 b1 ha iha hb ihb []//=.
+    move => [] //= t t0 ξ [*]. subst.
+    specialize iha with (1 := eq_refl).
+    specialize ihb with (1 := eq_refl).
+    move : iha => [a][? ?]. subst.
+    move : ihb => [b][? ?]. subst.
+    eexists. split.
+    by eauto using  P_LetBox.
+    by asimpl.
+  - hauto q:on ctrs:Par inv:Tm.
+  - hauto q:on ctrs:Par inv:Tm.
+Qed.
